theories/Math/ClassicalDomainTheory.v
@@ -7,7 +7,7 @@ Require Import DschingisKhan.Logic.ScottTopology.
 
 Module BasicCpoTheory.
 
-  Import MathProps MathClasses BasicPosetTheory BasicGeneralTopology DomainTheoryHelper ScottTopology.
+  Import MathProps MathClasses BasicPosetTheory BasicGeneralTopology DomainTheoryHelper ScottTopology ExclusiveMiddle.
 
   Definition ScottContinuousMaps (dom : Type) (cod : Type) {dom_requiresPoset : isPoset dom} {cod_requiresPoset : isPoset cod} : Type :=
     @sig (Hask.arrow dom cod) (isContinuousMap (dom_isTopology := TopologyOfDanaScott dom) (cod_isTopology := TopologyOfDanaScott cod))
@@ -28,34 +28,24 @@ Module BasicCpoTheory.
   Proof. (* Thanks to Junyoung Jang *)
     split.
     - intros y z y_in_U_x y_le_z z_le_x. unnw. contradiction y_in_U_x. now transitivity (z).
-    - intros X X_nonempty X_isDirected sup_X sup_X_isSupremumOf_X sup_X_in_U_x. unnw.
-      assert (JunyoungJang'sAdvice : ~ << UPPER_BOUND : forall z : D, member z X -> z =< x >>).
+    - intros X [X_nonempty X_isDirected] sup_X sup_X_isSupremumOf_X sup_X_in_U_x. unnw.
+      assert (NOT_UPPER_BOUND: ~ << UPPER_BOUND : forall z : D, member z X -> z =< x >>).
       { intros UPPER_BOUND. contradiction sup_X_in_U_x. now eapply sup_X_isSupremumOf_X. }
-      eapply ExclusiveMiddle.NNPP. intros H_false. contradiction JunyoungJang'sAdvice. intros y y_in_X.
-      eapply ExclusiveMiddle.NNPP. intros y_in_U_x. contradiction H_false. now exists (y).
+      eapply NNPP. intros H_false. contradiction NOT_UPPER_BOUND. intros y y_in_X.
+      eapply NNPP. intros y_in_U_x. contradiction H_false. now exists (y).
   Qed.
 
   Lemma ContinuousMap_isMonotonicMap {dom : Type} {cod : Type} {dom_isPoset : isPoset dom} {cod_isPoset : isPoset cod} (f : dom -> cod)
     (f_isContinuousMap : isContinuousMap f)
     : isMonotonicMap f.
   Proof.
-    intros x1 x2 x1_le_x2. eapply ExclusiveMiddle.NNPP. intros f_x1_in_U_f_x2.
+    intros x1 x2 x1_le_x2. eapply NNPP. intros f_x1_in_U_f_x2.
     assert (x1_in_preimage_f_U_f_x2 : member x1 (preimage f (U (f x2)))) by now econstructor.
     assert (preimage_f_U_f_x2_isOpen : isOpen (preimage f (U (f x2)))) by eapply f_isContinuousMap, U_x_isOpen.
     assert (x2_in_preimage_f_U_f_x2 : member x2 (preimage f (U (f x2)))).
     { inversion preimage_f_U_f_x2_isOpen. eapply UPWARD_CLOSED with (x := x1); eauto. }
     assert (f_x2_in_U_f_x2 : member (f x2) (U (f x2))) by now inversion x2_in_preimage_f_U_f_x2; subst.
     now contradiction f_x2_in_U_f_x2.
-  Qed.
-
-  Lemma MonotonicMap_preservesDirected {dom : Type} {cod : Type} {dom_isPoset : isPoset dom} {cod_isPoset : isPoset cod} (f : dom -> cod) (X : ensemble dom)
-    (f_isMonotonicMap : isMonotonicMap f)
-    (X_isDirected : isDirectedSubset X)
-    : isDirectedSubset (image f X).
-  Proof.
-    ii; desnw. apply in_image_iff in H_IN1, H_IN2. des.
-    pose proof (X_isDirected x0 H1 x H0) as [? [? [? ?]]]; unnw.
-    eexists; unnw. split; eauto. econstructor; eauto.
   Qed.
 
 End BasicCpoTheory.
